(WIP) likely wrong definitions of flattenX they do the flattening and then filter... e.g. (set x <- flatten(soup) | outside(x,pivot) rather than set x <- soup, y <- flatten(x) | outside(x, pivot)

Ownership.dfy
@@ -62,7 +62,8 @@ lemma OffsideIsSideways(part : Object, whole : Object)
  //important bit is that we don't *just want these offsiders*4
  //we *also* want any "outsiders" that are reachable without going through the pivot / the whole
  //see point below
-  ensures offside(part, whole) == (outside(part,whole) && not(inside(whole,part)))
+  ensures offside(part, whole) ==  (outside(part,whole) && not(inside(whole,part)))
+  ensures offside(part, whole) ==> (outside(part,whole))
 {}
 
 lemma STRICTLY_COME_INSIDE(part : Object, whole : Object)
@@ -75,6 +76,23 @@ lemma STRICTLY_COME_INSIDE(part : Object, whole : Object)
    ensures not(strictlyInside(part, whole)) <==> not(inside(part, whole) && (part != whole))
    ensures not(strictlyInside(part, whole)) <==>   (outside(part, whole) || (part == whole))
    ensures outside(part,whole) != inside(part,whole)
+{
+  assume part.Ready();
+  assume whole.Ready();
+}
+
+
+
+lemma PIVOTLY_COME_OUTSIDE(part : Object, whole : Object)
+  // requires part.Ready()
+  // requires whole.Ready()
+   ensures     pivotlyOutside(part, whole)  <==>    (outside(part, whole) || (part == whole))
+   ensures not(pivotlyOutside(part, whole)) <==> not(outside(part, whole) || (part == whole))
+
+   ensures     outside(part, whole)  <==>    (pivotlyOutside(part, whole) && (part != whole))
+   ensures not(outside(part, whole)) <==> not(pivotlyOutside(part, whole) && (part != whole))
+   ensures not(outside(part, whole))  <==>   (strictlyInside(part, whole) || (part == whole))
+   ensures strictlyInside(part,whole) != pivotlyOutside(part,whole)
 {
   assume part.Ready();
   assume whole.Ready();
@@ -107,6 +125,9 @@ lemma STRICTLY_COME_INSIDE(part : Object, whole : Object)
 
 lemma HappyFamilies0(next : Object, whole : Object)
   requires next.Ready()
+   ensures (allInside(next.AMFO, whole) + allOutside(next.AMFO, whole)) == next.AMFO
+   ensures (allInside({next}, whole) + allOutside({next}, whole)) == {next}
+
    ensures (allInside(next.AMFO, whole) + allOutside(next.AMFO, whole) + allOffside(next.AMFO, whole)) == next.AMFO
    ensures (allInside({next}, whole) + allOutside({next}, whole) + allOffside({next}, whole)) == {next}
 {
@@ -118,7 +139,9 @@ lemma HappyFamilies(soup : set<Object>, whole : Object, ins: set<Object>, outs: 
   requires ins   == allInside(soup, whole)
   requires outs  == allOutside(soup, whole)
   requires sides == allOffside(soup, whole)
+   ensures soup  == ins + outs
    ensures soup  == ins + outs + sides
+   ensures soup  >= outs >= sides
 {}
 
 //[[[[[[[[[[[[[[[[[[[[[[[[[[[[[[[[[[[[[[[[]]]]]]]]]]]]]]]]]]]]]]]]]]]]]]]]]]]]]]]]
@@ -253,29 +276,298 @@ lemma FLATTEN2(os : Owner, ps : Owner, fs : Owner)
    ensures flatten(os) + flatten(ps) == flatten(fs)
   {}
 
-function flattenInside(ownrs : OWNR, pivot : Object) : (rv : Owner)
+lemma FLATTEN9(os : Owner, fs : Owner)
+ decreases allAMFOs(os)
+  requires fs == flatten(os)
+   ensures fs == (set s <- os, f <- s.AMFO :: f) + os
+{}
+
+
+///Oh SHIT 0 most of the these are WRONG.
+
+ function flattenInside(soup : OWNR, pivot : Object) : (rv : Owner)
   ensures forall r <- rv :: inside(r,pivot)
-  ensures forall r <- flatten(ownrs) :: inside(r,pivot) ==> r in rv
-{ set x <- flatten(ownrs) | inside(x,pivot) }
+  ensures forall r <- flatten(soup) :: inside(r,pivot) ==> r in rv
+{ set x <- flatten(soup) | inside(x,pivot) }
 
-
-function flattenOutside(ownrs : OWNR, pivot : Object) : (rv : Owner)
+function flattenOutside(soup : OWNR, pivot : Object) : (rv : Owner)
   ensures forall r <- rv :: outside(r,pivot)
-  ensures forall r <- flatten(ownrs) :: outside(r,pivot) ==> r in rv
-{ set x <- flatten(ownrs) | outside(x,pivot) }
+  ensures forall r <- flatten(soup) :: outside(r,pivot) ==> r in rv
+{ set x <- flatten(soup) | outside(x,pivot) }
 
-
-function flattenOffside(ownrs : OWNR, pivot : Object) : (rv : Owner)
+function flattenOffside(soup : OWNR, pivot : Object) : (rv : Owner)
   ensures forall r <- rv :: offside(r,pivot)
-  ensures forall r <- flatten(ownrs) :: offside(r,pivot) ==> r in rv
-{ set x <- flatten(ownrs) | offside(x,pivot) }
+  ensures forall r <- flatten(soup) :: offside(r,pivot) ==> r in rv
+{ set x <- flatten(soup) | offside(x,pivot) }
 
-
-function flattenStrictlyInside(ownrs : OWNR, pivot : Object) : (rv : Owner)
+function flattenStrictlyInside(soup : OWNR, pivot : Object) : (rv : Owner)
   ensures forall r <- rv :: strictlyInside(r,pivot)
-  ensures forall r <- flatten(ownrs) :: strictlyInside(r,pivot) ==> r in rv
-{ set x <- flatten(ownrs) | strictlyInside(x,pivot) }
+  ensures forall r <- flatten(soup) :: strictlyInside(r,pivot) ==> r in rv
+{ set x <- flatten(soup) | strictlyInside(x,pivot) }
 
+function flattenPivotlyOutside(soup : OWNR, pivot : Object) : (rv : Owner)
+  ensures forall r <- rv :: pivotlyOutside(r,pivot)
+  ensures forall r <- flatten(soup) :: pivotlyOutside(r,pivot) ==> r in rv
+{ set x <- flatten(soup) | pivotlyOutside(x,pivot) }
+
+predicate onlyPivot(part : Object, pivot : Object, owner : Object) : (rv : bool)   reads {}   { inside(part, pivot) && inside(part,owner) &&  inside(pivot, owner) } // aka inside3(part,pivot,owner)
+predicate exceptPivot(part : Object, pivot : Object, owner : Object) : (rv : bool) reads {}   { inside(part, pivot) && inside(part,owner) && outside(pivot, owner) }
+   //should we explicitly require owner in part.AMFO  aka part inside owner?
+   //well apart from the "preconditions to the preconditions" problem
+
+function shortcutOnlyPivot(soup : OWNR, pivot : Object) : (rv : Owner)
+  ensures forall p <- pivot.AMFO :: inside(pivot, p)
+  ensures forall r <- rv :: inside(pivot, r)
+  ensures (rv == {}) != (rv == pivot.AMFO)
+  ensures (forall s <- soup :: outside(s,pivot)) ==> (rv == {})
+  ensures (exists s <- soup ::  inside(s,pivot)) ==> (rv == pivot.AMFO)
+  ensures forall r <- rv :: inside(pivot, r)
+  ensures forall r <- rv :: exists s <- soup :: onlyPivot(s, pivot, r)
+  ensures forall r <- rv :: r.Ready()
+  { assume forall s <- soup :: s.Ready(); assume pivot.Ready();
+    if (exists s <- soup :: inside(s,pivot)) then (pivot.AMFO) else {} }
+
+function flattenOnlyPivot(soup : OWNR, pivot : Object)  : (rv : Owner)
+ {set s <- soup, oo <- s.AMFO | onlyPivot(s,pivot,oo) :: oo}
+
+function flattenExceptPivot(soup : OWNR, pivot : Object) : (rv : Owner)
+ {set s <- soup, oo <- s.AMFO | exceptPivot(s,pivot,oo) :: oo}
+
+
+
+
+lemma LEMMA_flattenOnlyPivot0(soup : OWNR, pivot : Object, rv : Owner)
+  requires forall s <- soup :: s.Ready()
+  requires pivot.Ready()
+  requires (rv == flattenOnlyPivot(soup, pivot))
+   ensures forall r <- rv :: inside(pivot, r)
+   ensures forall r <- rv :: exists s <- soup :: onlyPivot(s,pivot,r)
+{}
+
+lemma LEMMA_flattenOnlyPivot1(soup : OWNR, pivot : Object, rv : Owner)
+  requires forall s <- soup :: s.Ready()
+  requires pivot.Ready()
+  requires (rv == flattenOnlyPivot(soup, pivot))
+
+  requires forall s <- soup :: outside(s,pivot)
+   ensures rv == {}
+{}
+
+lemma LEMMA_flattenOnlyPivot2(soup : OWNR, pivot : Object, rv : Owner)
+  requires forall s <- soup :: s.Ready()
+  requires pivot.Ready()
+  requires (rv == flattenOnlyPivot(soup, pivot))
+
+  requires exists s <- soup ::  inside(s,pivot)
+   ensures rv <= pivot.AMFO
+{
+  var s :| s in soup && inside(s,pivot);
+
+  forall r <- rv ensures (r in pivot.AMFO) //by
+   {
+      assert inside(pivot,r);
+      AXIOMAMFOREVERSE(pivot, r);
+   }
+  assert rv <= pivot.AMFO;
+}
+
+lemma LEMMA_flattenOnlyPivot3(soup : OWNR, pivot : Object, rv : Owner)
+  requires forall s <- soup :: s.Ready()
+  requires pivot.Ready()
+  requires (rv == flattenOnlyPivot(soup, pivot))
+
+  requires exists s <- soup ::  inside(s,pivot)
+   ensures rv >= pivot.AMFO
+{
+   var s :| s in soup && inside(s,pivot);
+   assert forall r <- s.AMFO     | onlyPivot(s,pivot,r) :: inside(pivot, r);
+   assert forall r <- s.AMFO     | onlyPivot(s,pivot,r) :: r in rv;
+
+   assert rv >= pivot.AMFO;
+}
+
+lemma LEMMA_flattenOnlyPivot9(soup : OWNR, pivot : Object, rv : Owner)
+  requires forall s <- soup :: s.Ready()
+  requires pivot.Ready()
+  requires (rv == flattenOnlyPivot(soup, pivot))
+   ensures (forall s <- soup :: outside(s,pivot)) ==> (rv == {})
+   ensures (exists s <- soup ::  inside(s,pivot)) ==> (rv == pivot.AMFO)
+{
+  if (forall s <- soup :: outside(s,pivot))
+     { LEMMA_flattenOnlyPivot1(soup,pivot,rv); return; }
+    else
+    { LEMMA_flattenOnlyPivot2(soup,pivot,rv); LEMMA_flattenOnlyPivot3(soup,pivot,rv); }
+}
+
+lemma LEMMA_shortcutOnlyPivot0(soup : OWNR, pivot : Object, rv : Owner)
+  requires forall s <- soup :: s.Ready()
+  requires pivot.Ready()
+  requires (rv == shortcutOnlyPivot(soup, pivot))
+
+   ensures forall r <- rv :: inside(pivot, r)
+   ensures forall r <- rv :: exists s <- soup :: inside(s,r)
+   ensures forall r <- rv :: inside(pivot, r) && (exists s <- soup :: inside(s,r))
+   ensures forall r <- rv :: exists s <- soup :: onlyPivot(s,pivot,r)
+{}
+
+lemma LEMMA_shortcutOnlyPivot1(soup : OWNR, pivot : Object, rv : Owner)
+  requires forall s <- soup :: s.Ready()
+  requires pivot.Ready()
+  requires (rv == shortcutOnlyPivot(soup, pivot))
+   ensures (forall s <- soup :: outside(s,pivot)) ==> (rv == {})
+   ensures (exists s <- soup ::  inside(s,pivot)) ==> (rv >  {})
+   ensures (exists s <- soup ::  inside(s,pivot)) ==> (rv == pivot.AMFO)
+{}
+
+lemma LEMMA_flattenExceptPivot0(soup : OWNR, pivot : Object, rv : Owner)
+  requires forall s <- soup :: s.Ready()
+  requires pivot.Ready()
+  requires (rv == flattenExceptPivot(soup, pivot))
+   ensures forall r <- rv :: outside(pivot,r) && (exists s <- soup :: inside(s,r))
+   ensures forall r <- rv :: exists s <- soup :: exceptPivot(s,pivot,r)
+   ensures forall r <- rv :: exists s <- soup :: inside(s, pivot) && inside(s,r) && outside(pivot, r)
+   //ensures forall r <- rv :: exists s <- soup :: exceptPivot(s,pivot,r) && pivotlyOutside(r,pivot)
+
+   ensures rv <= flatten(soup)
+   //  ensures (forall s <- soup :: outside(s,pivot) ==> (s in rv))
+  //  ensures (forall s <- soup, oo <- s.AMFO, ooo <- oo.AMFO | outside(ooo,pivot) :: (ooo in rv))
+   // ensures (rv == {}) ==> (forall s <- soup, oo <- s.AMFO :: colinear(oo.AMFO,pivot.AMFO))
+{
+  if (rv == {}) { return; }
+
+  var s :| s in soup && inside(s,pivot);
+  assert forall r <- s.AMFO     | exceptPivot(s,pivot,r) :: r in rv;
+
+
+}
+
+lemma LEMMA_shortcutVSflatten2(soup : OWNR, pivot : Object, shOP : Owner, fOP : Owner)
+  requires forall s <- soup :: s.Ready()
+  requires pivot.Ready()
+  requires shOP == shortcutOnlyPivot(soup, pivot)
+  requires fOP == flattenOnlyPivot(soup, pivot)
+  requires forall r <- shOP :: r.Ready()
+  requires forall r <- fOP  :: r.Ready()
+   ensures shOP == fOP
+   ensures (shOP == fOP == {}) || (shOP == fOP == pivot.AMFO)
+{
+  if (forall s <- soup :: not(inside(s,pivot)))
+    { assert shOP == fOP == {}; return; }
+
+  assert exists s <- soup :: inside(s,pivot);
+  LEMMA_flattenOnlyPivot9(soup,pivot,fOP);
+  assert shOP == fOP == pivot.AMFO;
+}
+
+
+lemma TRICHOTOMY_ONLY_EXCEPT(part : Object, pivot : Object, owner : Object)
+   ensures   onlyPivot(part,pivot,owner) ==> inside(part,pivot)
+   ensures exceptPivot(part,pivot,owner) ==> inside(part,pivot)
+  //  ensures      inside(part, pivot) ==> (onlyPivot(part,pivot,owner)
+  //                exceptPivot(part,pivot,owner))
+
+   ensures     outside(part, pivot) ==> (onlyPivot(part,pivot,owner) == exceptPivot(part,pivot,owner) == false)
+{
+  assume part.Ready();
+  assume pivot.Ready();
+  assume owner.Ready();
+}
+
+
+// inside(part, pivot) && inside(part,owner) &&  inside(pivot, owner)
+// inside(part, pivot) && inside(part,owner) && outside(pivot, owner)
+
+
+lemma OWNERZ_OF_PIVOTRY(soup : set<Object>, pivot : Object, fEP : Owner, fOP : Owner)
+ requires forall s <- soup :: s.Ready()
+ requires pivot.Ready()
+ requires fEP == flattenExceptPivot(soup,pivot)
+ requires fOP == flattenOnlyPivot(soup,pivot)
+  ensures forall r <- fEP :: exists s <- soup :: exceptPivot(s,pivot,r)
+  ensures forall r <- fOP :: exists s <- soup ::   onlyPivot(s,pivot,r)
+  ensures forall r <- fEP :: exists s <- soup :: exceptPivot(s,pivot,r)
+  ensures forall r <- fOP :: exists s <- soup ::   onlyPivot(s,pivot,r)
+    {}
+
+
+//////////////////////////////////////////////////////////////////////////////////////////////////////////////////
+// pivotlyOutside - pivotlyOutside(x,pivot)
+//   onlyPivot -  inside(pivot,owner)
+//   exceptPivot -outside(pivot,owner)
+lemma FUCKING_WIT_DA_PIVOT(pivot : Object, owner : Object)
+  requires pivot.Ready()
+  requires owner.Ready()
+    ensures pivotlyOutside(owner,pivot) == not(owner.AMFO > pivot.AMFO)
+    ensures  inside(pivot,owner) == (pivot.AMFO >= owner.AMFO)
+    ensures outside(pivot,owner) == not(pivot.AMFO >= owner.AMFO)
+
+    ensures    (pivot.AMFO >= owner.AMFO) ==> not(owner.AMFO > pivot.AMFO)
+    ensures           inside(pivot,owner) ==> pivotlyOutside(owner,pivot)
+//    ensures outside(pivot, owner) ==> pivotlyOutside(owner,pivot)
+//  ensures not(pivot.AMFO >= owner.AMFO) ==> not(owner.AMFO > pivot.AMFO)
+    {}
+
+
+//////////////////////////////////////////////////////////////////////////////////////////////////////////////////
+
+
+
+lemma FUCKING_WIT_pivotlyOutside(a : Object, b : Object)
+  requires a.Ready()
+  requires b.Ready()
+  requires pivotlyOutside(a,b)
+   ensures not(a.AMFO > b.AMFO)
+   ensures (a.AMFO == b.AMFO) || not(a.AMFO >= b.AMFO)
+    {}
+
+lemma FUCKING_WIT_DA_except_PIVOT(a : Object, b : Object, c : Object)
+  requires a.Ready()
+  requires b.Ready()
+  requires c.Ready()
+
+  requires exceptPivot(a,b,c)
+    ensures inside(a, b) && inside(a,c) && outside(b, c)
+    ensures (a.AMFO >= b.AMFO) && (a.AMFO >= c.AMFO) && not(b.AMFO >= c.AMFO)
+    ensures not(c.AMFO > b.AMFO)
+  //  ensures pivotlyOutside(c,b)
+    {}
+
+
+
+lemma TRICHOTOMY_DICHOTOMY(soup : Owner, pivot : Object, left0 : Owner, left1 : Owner, right : Owner)
+ requires forall s <- soup :: s.Ready()
+ requires pivot.Ready()
+ requires left0 == flattenStrictlyInside(soup,pivot)
+ requires left1 == flattenPivotlyOutside(soup,pivot)
+ requires right == flatten(soup)
+
+  ensures left0 <= right
+  ensures left1 <= right
+  ensures left0 + left1 <= right
+  ensures left0 + left1 >= right
+  ensures left0 + left1 == right
+ {}
+
+
+
+
+lemma DICHOTOMY_TRICHOTOMY(soup : Owner, pivot : Object, left0 : Owner, left1 : Owner, right : Owner)
+ requires forall s <- soup :: s.Ready()
+ requires pivot.Ready()
+ requires left0 == flattenExceptPivot(soup,pivot)
+ requires left1 == flattenOnlyPivot(soup,pivot)
+ requires right == flattenPivotlyOutside(soup,pivot)
+
+  ensures left0 <= right
+  ensures left1 <= right
+//  ensures left0 + left1 <= right
+  // ensures left0 + left1 >= right
+  // ensures left0 + left1 == right
+
+///HERE///
+
+{
+}
 
 
 //From DAHLIA
